Machines.lean
@@ -21,8 +21,6 @@ import Machines.Lnp64u.Logic.SystemOpsWf
 import Machines.Lnp64u.Logic.Sep.Resource
 import Machines.Tutorial.SatCounter
 import Machines.Multiclock.TwoCounters
-import Machines.Tutorial.SatCounter
-import Machines.Multiclock.TwoCountersArtifact
 import Machines.Substrate.S0Blinky
 import Machines.Substrate.S13Soak
 import Machines.Substrate.S0BscanRegs
